Updating PSS and RandomOracle. RandomOracle should become the default random oracle formalization once we're sure it is sufficient.

examples/RandomOracle.ec
@@ -10,20 +10,22 @@ theory Types.
   (* A signature for random oracles from "from" to "to". *)
   module type Oracle =
   {
-    fun init():unit {*}
-    fun o(x:from):to
+    proc * init():unit
+    proc o (x:from):to
   }.
 
-  module type ARO = { fun o(x:from):to }.
+  module type ARO = {
+    proc o(x:from):to
+  }.
 
   module type Dist (H:ARO) = {
-    fun distinguish(): bool {* H.o}
+    proc * distinguish(): bool
   }.
 
   module IND(H:Oracle,D:Dist) = {
     module D = D(H)
 
-    fun main(): bool = {
+    proc main(): bool = {
       var b:bool;
 
       H.init();
@@ -48,11 +50,11 @@ theory Lazy.
   module RO:Oracle = {
     var m:(from, to) map
 
-    fun init():unit = {
+    proc init():unit = {
       m = FMap.Core.empty;
     }
   
-    fun o(x:from):to = {
+    proc o(x:from):to = {
       var y:to;
       y = $dsample x;
       if (!in_dom x m) m.[x] = y;
@@ -62,23 +64,23 @@ theory Lazy.
 
   lemma lossless_init: islossless RO.init.
   proof strict.
-  by fun; wp.
+  by proc; wp.
   qed.
 
   lemma lossless_o:
     (forall x, mu (dsample x) cpTrue = 1%r) =>
     islossless RO.o.
   proof strict.
-  by intros=> dsampleL; fun; wp; rnd; skip; smt.
+  by intros=> dsampleL; proc; wp; rnd; skip; smt.
   qed.
 
   equiv abstract_init:
     RO.init ~ RO.init: true ==> ={glob RO}
-  by (fun; wp).
+  by (proc; wp).
 
   equiv abstract_o:
     RO.o ~ RO.o: ={glob RO, x} ==> ={glob RO, res}
-  by (fun; eqobs_in).
+  by (proc; sim).
 end Lazy.
 
 theory Eager.
@@ -99,7 +101,7 @@ theory Eager.
   module RO: Oracle = {
     var m:(from,to) map
 
-    fun init(): unit = {
+    proc init(): unit = {
       var y:to;
       var work:from set;
       var f:from;
@@ -115,7 +117,7 @@ theory Eager.
       }
     }
 
-    fun o(x:from): to = {
+    proc o(x:from): to = {
       return proj m.[x];
     }
   }.
@@ -125,7 +127,7 @@ theory Eager.
     (forall x, mu (dsample x) cpTrue = 1%r) =>
     islossless RO.init.
   proof strict.
-  intros=> fType dsampleL; fun.
+  intros=> fType dsampleL; proc.
   while (true) (card work).
     by intros=> z; wp; rnd cpTrue; wp;
        skip; smt.
@@ -134,21 +136,21 @@ theory Eager.
 
   lemma lossless_o: islossless RO.o.
   proof strict.
-  by fun; wp.
+  by proc; wp.
   qed.
 
   lemma abstract_init:
     finite univ<:from> =>
     equiv [RO.init ~ RO.init: true ==> ={glob RO} /\ forall x, in_dom x RO.m{1}].
   proof strict.
-  intros=> fType; fun;
+  intros=> fType; proc;
   while (={glob RO, work} /\ forall x, !mem x work{1} => in_dom x RO.m{1}).
     by wp; rnd; wp; skip; progress=> //; smt.
   by wp; skip; smt.
   qed.
 
   equiv abstract_o: RO.o ~ RO.o: ={glob RO, x} ==> ={glob RO, res}
-  by (fun; wp).
+  by (proc; wp).
 end Eager.
 
 theory LazyEager.
@@ -179,18 +181,17 @@ theory LazyEager.
     op dsample <- dsample.
 
   section.
-  (* Proof note: We may be missing losslessness assumptions on D *)
   declare module D:Dist {Lazy.RO,Eager.RO}.
 
   local module IND_Lazy = {
     module H:Oracle = {
       var m:(from, to) map
 
-      fun init():unit = {
+      proc init():unit = {
         m = FMap.Core.empty;
       }
   
-      fun o(x:from):to = {
+      proc o(x:from):to = {
         var y:to;
         y = $dsample x;
         if (!in_dom x m) m.[x] = y;
@@ -198,7 +199,7 @@ theory LazyEager.
       }
     }
 
-    fun resample(): unit = {
+    proc resample(): unit = {
       var work:from set;
       var f:from;
       var y,y0:to;
@@ -215,7 +216,7 @@ theory LazyEager.
 
     module D = D(H)
 
-    fun main(): bool = {
+    proc main(): bool = {
       var b:bool;
 
       H.init();
@@ -229,10 +230,10 @@ theory LazyEager.
   local lemma IND_Lazy: (forall x, mu (dsample x) cpTrue = 1%r) =>
     equiv [IND(Lazy.RO,D).main ~ IND_Lazy.main: true ==> ={res}].
   proof strict.
-  intros=> dsampleL; fun; seq 2 2: (={b}).
-    call (_: Lazy.RO.m{1} = IND_Lazy.H.m{2}); first by fun; eqobs_in.
+  intros=> dsampleL; proc; seq 2 2: (={b}).
+    call (_: Lazy.RO.m{1} = IND_Lazy.H.m{2}); first by (proc; sim).
     by call (_: true ==> Lazy.RO.m{1} = IND_Lazy.H.m{2})=> //;
-      first by fun; wp.
+      first by proc; wp.
     inline IND_Lazy.resample;
     while{2} (true) (card work{2}).
       intros=> &m z; wp; rnd; wp; skip; progress=> //; last smt.
@@ -244,12 +245,12 @@ theory LazyEager.
     module H = {
       var m:(from,to) map
 
-      fun o(x:from): to = {
+      proc o(x:from): to = {
         return proj (m.[x]);
       }
     }
 
-    fun resample(): unit = {
+    proc resample(): unit = {
       var work:from set;
       var f:from;
       var y,y0:to;
@@ -266,7 +267,7 @@ theory LazyEager.
 
     module D = D(H)
 
-    fun main(): bool = {
+    proc main(): bool = {
       var b:bool;
 
       H.m = FMap.Core.empty;
@@ -284,7 +285,7 @@ theory LazyEager.
       ={x} /\ IND_Eager.H.m{1} = IND_Lazy.H.m{2} ==>
       ={res} /\ IND_Eager.H.m{1} = IND_Lazy.H.m{2}].
   proof strict.
-  intros=> dsampleL; eager fun.
+  intros=> dsampleL; eager proc.
   inline IND_Eager.resample IND_Lazy.resample; swap{2} 4 -3.
   seq 1 1: (={x,work} /\
             IND_Eager.H.m{1} = IND_Lazy.H.m{2} /\
@@ -320,14 +321,14 @@ theory LazyEager.
                      (={x,work,IND_Eager.H.m} ==> ={result,IND_Eager.H.m})
                      (={x,work,IND_Eager.H.m} ==> ={result,IND_Eager.H.m})=> //.
       by intros &1 &2 H; exists IND_Eager.H.m{2}, x{2}, work{2}; generalize H.
-    by eqobs_in; rnd{2}; eqobs_in true true: (={x,IND_Eager.H.m}); smt.
+    by sim; rnd{2}; sim true true: (={x,IND_Eager.H.m}); smt.
 
     wp; symmetry.
     eager while (H:y0 = $dsample x; ~ y0 = $dsample x; : ={x} ==> ={y0})=> //; first by rnd.
       swap{2} 5 -4; swap [2..3] -1; case (x = pick work){1}.
         by wp; rnd{2}; rnd; rnd{1}; wp; skip; smt.
         by wp; do 2!rnd; wp; skip; smt.
-      by eqobs_in.
+      by sim.
 
     wp; while (={x, work} /\
                (!mem x work => in_dom x IND_Eager.H.m){1} /\
@@ -335,7 +336,7 @@ theory LazyEager.
                if (in_dom x IND_Eager.H.m){1}
                  then IND_Eager.H.m{1} = IND_Lazy.H.m{2}
                  else eq_except IND_Eager.H.m{1} IND_Lazy.H.m{2} x{1}).
-      by wp; rnd; wp; skip; progress=> //; try case (pick work = x){2}; smt.
+      wp; rnd; wp; skip; progress=> //; try case (pick work = x){2}; smt.
     by wp; rnd; skip; progress=> //; smt.
 
   wp; while (={x,work} /\
@@ -349,27 +350,27 @@ theory LazyEager.
   local lemma eager_aux: (forall x, mu (dsample x) cpTrue = 1%r) =>
     equiv [IND_Lazy.main ~ IND_Eager.main: true ==> ={res}].
   proof strict.
-  intros=> dsampleL; fun; inline IND_Lazy.H.init.
+  intros=> dsampleL; proc; inline IND_Lazy.H.init.
   seq 1 1: (IND_Lazy.H.m{1} = IND_Eager.H.m{2}); first by wp.
   symmetry;
   eager (H: IND_Eager.resample(); ~ IND_Lazy.resample();:
               IND_Eager.H.m{1} = IND_Lazy.H.m{2} ==> IND_Eager.H.m{1} = IND_Lazy.H.m{2}): 
         (IND_Eager.H.m{1} = IND_Lazy.H.m{2})=> //;
-    first by eqobs_in.
-  eager fun H (IND_Eager.H.m{1} = IND_Lazy.H.m{2})=> //;
+    first by sim.
+  eager proc H (IND_Eager.H.m{1} = IND_Lazy.H.m{2})=> //;
     first by apply eager_query=> //.
-  by fun; eqobs_in.
+  by proc; sim.
   qed.
 
   local lemma IND_Eager: (forall x, mu (dsample x) cpTrue = 1%r) =>
     equiv [IND_Eager.main ~ IND(Eager.RO,D).main: true ==> ={res}].
   proof strict.
-  intros=> dsampleL; fun.
+  intros=> dsampleL; proc.
   call (_: (forall x, in_dom x IND_Eager.H.m{1}) /\ IND_Eager.H.m{1} = Eager.RO.m{2}).
-    by fun; skip; smt.
+    by proc; skip; smt.
   inline RO.init IND_Eager.resample.
     while (={work} /\ (forall x, !in_dom x IND_Eager.H.m{1} <=> mem x work{1}) /\ IND_Eager.H.m{1} = Eager.RO.m{2}).
-      wp; rnd; wp; skip; progress=> //; smt.
+      by wp; rnd; wp; skip; progress=> //; smt.
     by wp; skip; smt.
   qed.
 
@@ -378,10 +379,10 @@ theory LazyEager.
   proof strict.
   intros=> dsampleL; bypr (res{1}) (res{2})=> //; intros=> &1 &2 a.
   apply (eq_trans _ Pr[IND_Lazy.main() @ &1: a = res]);
-    first by equiv_deno (IND_Lazy _).
+    first by byequiv (IND_Lazy _).
   apply (eq_trans _ Pr[IND_Eager.main() @ &1: a = res]);
-    first by equiv_deno (eager_aux _).
-  by equiv_deno (IND_Eager _).
+    first by byequiv (eager_aux _).
+  by byequiv (IND_Eager _).
   qed.
   end section.
 end LazyEager.
@@ -394,14 +395,14 @@ theory Wrappers.
     op dsample = dsample.
 
   module type WRO = {
-    fun init(qO:int): unit {*}
-    fun o(x:from): to
+    proc * init(qO:int): unit {}
+    proc o(x:from): to
   }.
 
   module IND_b(H:WRO,D:Dist) = {
     module D = D(H)
 
-    fun main(qO:int): bool = {
+    proc main(qO:int): bool = {
       var b:bool;
       H.init(qO);
       b = D.distinguish();
@@ -415,13 +416,13 @@ theory Wrappers.
     var qO:int
     var qs:int
 
-    fun init(qO:int): unit = {
+    proc init(qO:int): unit = {
       H.init();
       Count.qO = qO;
       qs = 0;
     }
 
-    fun o(x:from): to = {
+    proc o(x:from): to = {
       var r:to;
       if (qs < qO)
       {
@@ -444,19 +445,19 @@ theory Wrappers.
                  ={res} /\
                  size Lazy.RO.m{1} <= Count.qs{2}) ].
   proof strict.
-  intros=> lt0_qO dsampleL DL; fun.
+  intros=> lt0_qO dsampleL DL; proc.
   call (_: Count.qO <= Count.qs,
            ={glob Lazy.RO} /\
            Count.qO{2} = qO' /\
            size Lazy.RO.m{1} <= Count.qs{2}).
     (* H *)
-    fun; rcondt{2} 1; first intros=> &m; skip; progress=> //; smt.
+    proc; rcondt{2} 1; first intros=> &m; skip; progress=> //; smt.
       inline Lazy.RO.o; wp; rnd; wp; skip; progress=> //; last smt.
         by rewrite /size dom_set card_add_nin -/(in_dom _ _); last smt.
     by intros=> _ _; apply Lazy.lossless_o.
-    by intros=> _; fun; if=> //; inline Lazy.RO.o; wp; rnd; wp; skip; smt.
+    by intros=> _; proc; if=> //; inline Lazy.RO.o; wp; rnd; wp; skip; smt.
   inline Count(Lazy.RO).init; wp; call (_: true ==> ={glob Lazy.RO} /\ dom Lazy.RO.m{1} = FSet.empty)=> //;
-    first by fun; wp; skip; progress=> //; smt.
+    first by proc; wp; skip; progress=> //; smt.
   wp; skip; cut H1: ISet.empty<:from> == FSet.empty by smt; progress=> //.
     by rewrite /size H card_empty.
     by cut [eq_res _]:= H2 _; first smt.
@@ -493,13 +494,13 @@ theory Wrappers.
     var qs:(from,int) map
     var qc:int
 
-    fun init(): unit = {
+    proc init(): unit = {
       H.init();
       qs = FMap.Core.empty;
       qc = 0;
     }
 
-    fun o(x:from): to = {
+    proc o(x:from): to = {
       var r:to;
       if (!in_dom x qs)
       {
